src/Nomega.v
@@ -1,0 +1,37 @@
+(* Make [omega] work for [N] *)
+
+Require Import Arith Omega NArith.
+
+Local Open Scope N_scope.
+
+Hint Rewrite Nplus_0_r nat_of_Nsucc nat_of_Nplus N_of_nat_of_N : N.
+
+Theorem nat_of_N_eq : forall n m,
+  nat_of_N n = nat_of_N m
+  -> n = m.
+  intros ? ? H; apply (f_equal N_of_nat) in H;
+    autorewrite with N in *; assumption.
+Qed.
+
+Theorem Nlt_out : forall n m, n < m
+  -> (nat_of_N n < nat_of_N m)%nat.
+  unfold Nlt; intros.
+  rewrite nat_of_Ncompare in H.
+  apply nat_compare_Lt_lt; assumption.
+Qed.
+
+Theorem Nlt_in : forall n m, (nat_of_N n < nat_of_N m)%nat
+  -> n < m.
+  unfold Nlt; intros.
+  rewrite nat_of_Ncompare.
+  apply (proj1 (nat_compare_lt _ _)); assumption.
+Qed.
+
+Ltac pre_nomega :=
+  try (apply nat_of_N_eq || apply Nlt_in); autorewrite with N;
+    repeat match goal with
+             | [ H : _ |- _ ] => (apply (f_equal nat_of_N) in H
+               || apply Nlt_out in H); autorewrite with N in H
+           end.
+
+Ltac nomega := pre_nomega; omega.
