src/Structured.v
@@ -1,0 +1,263 @@
+(* Structured programming *)
+
+Require Import NArith String List.
+
+Require Import Nomega PropX PropXTac Word LabelMap IL XCAP.
+
+Set Implicit Arguments.
+
+Local Open Scope N_scope.
+
+
+Section imports.
+  (* Which external code labels must be available? *)
+  Variable imports : LabelMap.t assert.
+
+  Hypothesis imports_global : forall k v, LabelMap.MapsTo k v imports
+    -> exists s, snd k = Global s.
+
+  (* Which code module are we defining here? *)
+  Variable modName : string.
+
+  (* Full set of code labels that may be mentioned in generated code *)
+  Fixpoint imps (bls : list (assert * block)) (base exit : N) (post : assert) : LabelMap.t assert :=
+    match bls with
+      | nil => LabelMap.add (modName, Local exit) post imports
+      | (pre, _) :: bls' => LabelMap.add (modName, Local base) pre (imps bls' (Nsucc base) exit post)
+    end.
+
+  (** The data type of structured program pieces *)
+
+  Record codeGen (Precondition : assert) (Base Exit : N) (Postcondition : assert) (VerifCond : Prop) := {
+    Entry : N;                      (* Jump here to start *)
+    Blocks : list (assert * block); (* Code blocks *)
+
+    PreconditionOk : exists pre, exists bl, nth_error Blocks (nat_of_N Entry) = Some (pre, bl)
+      /\ forall specs stn st, interp specs (Precondition stn st)
+        -> interp specs (pre stn st);
+    
+    BlocksOk : VerifCond
+      -> Exit < Base
+      -> List.Forall (fun p => blockOk (imps Blocks Base Exit Postcondition) (fst p) (snd p)) Blocks
+  }.
+
+  Record codeOut (Precondition : assert) := {
+    Postcondition : assert;     (* Guarantee this on exit. *)
+    VerifCond : Prop;           (* User must prove this *)
+    Generate : forall Base Exit : N, (* Start generating code labels at this address *)
+      codeGen Precondition Base Exit Postcondition VerifCond
+  }.
+
+  Inductive cmd :=
+  | StraightLine : list instr -> cmd
+  | Structured : (forall ci, codeOut ci) -> cmd.
+
+
+  (** Sequencing *)
+
+  Definition notStuck (pre : assert) (is : list instr) :=
+    forall stn st specs, interp specs (pre stn st)
+      -> evalInstrs stn st is <> None.
+
+  Lemma lookup_imps : forall p bl exit post bls n base,
+    nth_error bls (nat_of_N n) = Some (p, bl)
+    -> LabelMap.MapsTo (modName, Local (Nsucc base + n)) p
+    (imps bls (Nsucc base) exit post).
+    induction bls; simpl in *; intuition.
+
+    destruct (nat_of_N n); discriminate.
+
+    induction n using Nind; simpl in *.
+
+    injection H; clear H; intros; subst.
+    autorewrite with N.
+    apply LabelMap.add_1; reflexivity.
+
+    autorewrite with N in *; simpl in *.
+    apply (IHbls n (Nsucc base)) in H.
+    apply LabelMap.add_2.
+    intro.
+    injection H0; clear H0; intros.
+    nomega.
+    
+    replace (Nsucc base + Nsucc n) with (Nsucc (Nsucc base) + n) by nomega.
+    assumption.
+  Qed.
+
+  Lemma lookup_imps_plus : forall {p bl exit post p' bls n base},
+    nth_error bls (nat_of_N n) = Some (p, bl)
+    -> LabelMap.MapsTo (modName, Local (Nsucc base + n)) p
+    (LabelMap.add (modName, Local base) p'
+      (imps bls (Nsucc base) exit post)).
+    intros.
+    apply LabelMap.add_2.
+
+    intro.
+    injection H0; clear H0; intros.
+    nomega.
+
+    eapply lookup_imps; eauto.
+  Qed.
+
+  Hint Resolve lookup_imps @lookup_imps_plus.
+  Hint Immediate simplify_fwd.
+
+  Lemma blockOk_impl : forall imps imps' p bl,
+    (forall k v, LabelMap.MapsTo k v imps
+      -> LabelMap.MapsTo k v imps')
+    -> blockOk imps p bl
+    -> blockOk imps' p bl.
+    unfold blockOk; intuition.
+    specialize (H0 stn specs).
+    match type of H0 with
+      | ?P -> _ => assert P by auto; intuition
+    end.
+    specialize (H4 _ H2); destruct H4; intuition.
+    destruct H5; intuition.
+    destruct H6; intuition.
+    eauto 8.
+  Qed.
+
+  Hint Resolve blockOk_impl.
+
+  Lemma imps_preserve : forall k v exit post n pre bls base,
+    LabelMap.MapsTo k v (imps bls base exit post)
+    -> n < base
+    -> exit < n
+    -> LabelMap.MapsTo k v (LabelMap.add (modName, Local n) pre
+        (imps bls base exit post)).
+    induction bls; simpl; intuition.
+
+    apply LabelFacts.add_mapsto_iff in H; intuition; subst.
+    apply LabelMap.add_2.
+    intro.
+    injection H; clear H; intros.
+    nomega.
+    apply LabelMap.add_1; reflexivity.
+
+    apply LabelMap.add_2.
+    apply imports_global in H3; destruct H3.
+    destruct k; simpl in *; congruence.
+    apply LabelMap.add_2.
+    apply imports_global in H3; destruct H3.
+    destruct k; simpl in *; congruence.
+    assumption.
+
+    apply LabelFacts.add_mapsto_iff in H; intuition; subst.
+    apply LabelMap.add_2.
+    intro.
+    injection H; clear H; intros.
+    nomega.
+    apply LabelMap.add_1; reflexivity.
+
+    specialize (IHbls _ H3).
+    assert (n < Nsucc base) by nomega; intuition.
+    apply LabelFacts.add_mapsto_iff in H5; intuition; subst.
+    apply LabelMap.add_1; reflexivity.
+    apply LabelMap.add_2; auto.
+    apply LabelMap.add_2; auto.
+  Qed.
+
+  Hint Resolve imps_preserve.
+
+  Lemma lt_succ : forall n, n < Nsucc n.
+    intros; nomega.
+  Qed.
+
+  Lemma lt_succ' : forall n m, n < m -> n < Nsucc m.
+    intros; nomega.
+  Qed.
+
+  Hint Immediate lt_succ lt_succ'.
+
+  Hint Extern 1 (List.Forall _ _) => eapply Forall_impl; [ | eassumption ].
+
+  Definition seq (c1 c2 : cmd) : cmd.
+    refine (match c1, c2 with
+              | StraightLine is1, StraightLine is2 => StraightLine (is1 ++ is2)
+
+              | StraightLine is, Structured cf =>
+                Structured (fun pre =>
+                  let cout := cf (fun stn st =>
+                    Ex st', [evalInstrs stn st' is = Some st] /\ pre stn st')%PropX in
+                  {|
+                    Postcondition := Postcondition cout;
+                    VerifCond := notStuck pre is /\ VerifCond cout;
+                    Generate := fun Base Exit =>
+                      let cg := Generate cout (Nsucc Base) Exit in
+                        {|
+                          Entry := 0;
+                          Blocks := (pre, (is, Uncond (RvLabel (modName, Local (Nsucc Base + Entry cg))))) :: Blocks cg
+                        |}
+                  |})
+
+              | Structured cf, StraightLine is =>
+                Structured (fun pre =>
+                  let cout := cf pre in
+                  {|
+                    Postcondition := (fun stn st =>
+                      Ex st', [evalInstrs stn st' is = Some st] /\ Postcondition cout stn st')%PropX;
+                    VerifCond := VerifCond cout /\ notStuck (Postcondition cout) is;
+                    Generate := fun Base Exit =>
+                      let cg := Generate cout (Nsucc Base) Base in
+                        {|
+                          Entry := Nsucc (Entry cg);
+                          Blocks := (Postcondition cout, (is, Uncond (RvLabel (modName, Local Exit)))) :: Blocks cg
+                        |}
+                  |})
+
+              | Structured cf1, Structured cf2 =>
+                Structured (fun pre =>
+                  let cout1 := cf1 pre in
+                  let cout2 := cf2 (Postcondition cout1) in
+                  {|
+                    Postcondition := Postcondition cout2;
+                    VerifCond := VerifCond cout1 /\ VerifCond cout2;
+                    Generate := fun Base Exit =>
+                      let cg2 := Generate cout2 Base Exit in
+                      let numBlocks := N_of_nat (length (Blocks cg2)) in
+                      let cg1 := Generate cout1 (Base + numBlocks) (Base + Entry cg2) in
+                        {|
+                          Entry := numBlocks + Entry cg1;
+                          Blocks := Blocks cg2 ++ Blocks cg1
+                        |}
+                  |})
+            end); simpl in *; intuition eauto; repeat (apply Forall_nil || apply Forall_cons); simpl.
+
+    Ltac simp := repeat (match goal with
+                           | [ x : codeGen _ _ _ _ _ |- _ ] => destruct x; simpl in *
+                           | [ H : ex _ |- _ ] => destruct H
+                           | [ H1 : notStuck _ _, H2 : _ |- _ ] => specialize (H1 _ _ _ H2)
+                           | [ H : _, H' : _ |- _ ] => specialize (H _ _ (lookup_imps_plus H')); destruct H; intuition
+                           | [ |- blockOk _ _ _ ] => red
+                           | [ H : ?E = None -> False |- _ ] => case_eq E; intros; tauto || clear H
+                           | [ H : _ |- _ ] => rewrite H
+                           | [ H : ?P -> _ |- _ ] =>
+                             match type of P with
+                               | Prop => assert P by auto; intuition
+                             end
+                         end; intuition; unfold evalBlock; simpl; autorewrite with N).
+    Ltac finisher := repeat match goal with
+                              | [ |- ex _ ] => esplit
+                              | [ |- _ /\ _ ] => split
+                              | [ H : _ |- interp _ _ ] => apply H; propxFo
+                            end; (instantiate; eauto).
+
+    Ltac t := simp; finisher.
+
+    t.
+    
+    t.
+
+    t.
+
+    admit.
+
+    admit.
+
+    admit.
+
+    admit.
+  Qed.
+
+End imports.
